denning-sacco-central-auth/DS.Debug.fst
@@ -69,12 +69,12 @@ let fake_cert_attacker () =
   let before_sigk_srv = global_timestamp () in
   let sigk_srv_idx = gen_private_key #ds_preds #before_sigk_srv auth_srv SIG "DS.sig_key" in
 
-  let before_pk_a = global_timestamp () in
-  let pk_a_srv_idx = install_public_key #ds_preds #before_pk_a a auth_srv SIG "DS.sig_key" in
+  let t_pk_a = global_timestamp () in
+  let pk_a_srv_idx = install_public_key #ds_preds #t_pk_a a auth_srv SIG "DS.sig_key" in
   let now = global_timestamp () in
   let pk_b_srv_idx = install_public_key #ds_preds #now b auth_srv PKE "DS.pke_key" in
-  let before_pk_e = global_timestamp () in
-  let pk_e_srv_idx = install_public_key #ds_preds #before_pk_e e auth_srv PKE "DS.pke_key" in
+  let t_pk_e = global_timestamp () in
+  let pk_e_srv_idx = install_public_key #ds_preds #t_pk_e e auth_srv PKE "DS.pke_key" in
   let now = global_timestamp () in
   let verk_srv_a_idx = install_public_key #ds_preds #now auth_srv a SIG "DS.sig_key" in
   let now = global_timestamp () in
@@ -82,34 +82,50 @@ let fake_cert_attacker () =
 
   // compromise eve's secret key
   let idx_comp_e = compromise e sk_e_idx 0 in
-  let now = global_timestamp () in
-  let sk_e = query_secret_key (before_sk_e + 1) idx_comp_e now e sk_e_idx 0 in
+  let after_comp_sk_e = global_timestamp () in
+  let sk_e = query_secret_key (before_sk_e + 1) idx_comp_e after_comp_sk_e e sk_e_idx 0 in
+  print_string "compromised eve's secret key\n";
 
-  // compromise server's secret key and pub keys of eve and alice
+  // compromise server's sign key and pub keys of eve and alice
   let idx_comp_srv = compromise auth_srv sigk_srv_idx 0 in
   let after_comp_sigk_srv = global_timestamp () in
   let sigk_srv = query_secret_key (before_sigk_srv + 1) idx_comp_srv after_comp_sigk_srv auth_srv sigk_srv_idx 0 in
+  print_string "compromised server's sign key\n";
 
   let idx_comp_srv = compromise auth_srv pk_e_srv_idx 0 in
   let after_comp_pk_e = global_timestamp () in
-  let pk_e = query_public_key (before_pk_e + 1) idx_comp_srv after_comp_pk_e auth_srv pk_e_srv_idx 0 in
+  let pk_e = query_public_key t_pk_e idx_comp_srv after_comp_pk_e auth_srv pk_e_srv_idx 0 in
+  print_string "queried eve's public key in server state\n";
 
   let idx_comp_srv = compromise auth_srv pk_a_srv_idx 0 in
   let after_comp_pk_a = global_timestamp () in
-  let pk_a = query_public_key (before_pk_a + 1) idx_comp_srv after_comp_pk_a auth_srv pk_a_srv_idx 0 in
+  let pk_a = query_public_key t_pk_a idx_comp_srv after_comp_pk_a auth_srv pk_a_srv_idx 0 in
+  print_string "queried alice's public key in server state\n";
 
   let sigk_srv = pub_bytes_later after_comp_sigk_srv after_comp_pk_a sigk_srv in
   let pk_e = pub_bytes_later after_comp_pk_e after_comp_pk_a pk_e in
+  let sk_e = pub_bytes_later after_comp_sk_e after_comp_pk_a sk_e in
 
   let (msg1_idx, a_sess_idx) = initiator_send_msg_1 a b in
-  let (|msg2_idx,c_out|) = attacker_issue_fake_cert e sigk_srv pk_a pk_e msg1_idx in
-  ()
+  let (|msg2_idx,c_sm2|) = attacker_issue_fake_cert e sigk_srv pk_a pk_e msg1_idx in
+  let (msg3_idx, c_sm3) = initiator_send_msg_3 c_sm2 a msg2_idx a_sess_idx in
+  let (|t_ck,ck,c_end|) = attacker_recv_msg_3 c_sm3 e sk_e msg3_idx in
+
+  print_bytes ck; print_string "\n";
+  attacker_knows_comm_key_stored_in_initiator_state a a_sess_idx ck
 
 let benign () : LCrypto unit (pki ds_preds)
   (requires (fun _ -> True)) (ensures (fun _ _ _ -> True))
 = print_string "start\n";
   let t0 = get () in
   let x = benign_attacker () in
+  print_trace ()
+
+let fake_cert () : LCrypto unit (pki ds_preds)
+  (requires (fun _ -> True)) (ensures (fun _ _ _ -> True))
+= print_string "start\n";
+  let t0 = get () in
+  let x = fake_cert_attacker () in
   print_trace ()
 
 let main =
@@ -123,4 +139,11 @@ let main =
   (match r with
   | Error s -> IO.print_string ("ERROR: "^s^"\n")
   | Success _ -> IO.print_string "PROTOCOL RUN: Successful execution of Denning-Sacco protocol.\n");
-  IO.print_string "Finished Benign Attacker:\n"
+  IO.print_string "Finished Benign Attacker:\n";
+  IO.print_string "Starting Fake Certificate Attacker:\n";
+  assume(valid_trace (pki ds_preds) t0);
+  let r,t1 = (reify (fake_cert ()) t0) in
+  (match r with
+  | Error s -> IO.print_string ("ERROR: "^s^"\n")
+  | Success _ -> IO.print_string "PROTOCOL RUN: Successful execution of Denning-Sacco protocol.\n");
+  IO.print_string "Finished Fake Certificate Attacker:\n"
